poSTVM/poSTVM_state_alt.thy
@@ -24,19 +24,25 @@ definition find_var_by_name :: "symbolic_var  \<Rightarrow>(symbolic_var, stacke
 "find_var_by_name var val =(fmlookup val var) "
 
 text "Getting var init from process vars by name"
-fun get_var_by_name :: "(stacked_proc_var list) \<Rightarrow>  symbolic_var \<Rightarrow>  stacked_var_init option" where
-  "get_var_by_name (x#yz) var_name  = (let res = (case x of stacked_proc_var.ProcessVar var \<Rightarrow> None |
-                                          stacked_proc_var.Var  var \<Rightarrow> find_var_by_name var_name var |
-                                          stacked_proc_var.InVar var \<Rightarrow> find_var_by_name var_name var | 
-                                          stacked_proc_var.OutVar var \<Rightarrow> find_var_by_name var_name var | 
-                                          stacked_proc_var.InOutVar var \<Rightarrow> find_var_by_name var_name var) 
+primrec get_var_by_name :: "(stacked_proc_var list) \<Rightarrow>  symbolic_var \<Rightarrow>  stacked_var_init option" where
+  "get_var_by_name [] _ = None"
+| "get_var_by_name (x#yz) var_name  =
+    (let res = 
+      (case x of 
+        stacked_proc_var.ProcessVar var \<Rightarrow> None 
+      | stacked_proc_var.Var  var \<Rightarrow> find_var_by_name var_name var 
+      | stacked_proc_var.InVar var \<Rightarrow> find_var_by_name var_name var 
+      | stacked_proc_var.OutVar var \<Rightarrow> find_var_by_name var_name var 
+      | stacked_proc_var.InOutVar var \<Rightarrow> find_var_by_name var_name var) 
     in (if res = None 
           then get_var_by_name yz var_name 
           else res))"
 
+print_theorems
+
 text "Getting current process state from program state"
-fun get_cur_proc_state_by_prog :: "program_state \<Rightarrow> process_state" where
-"get_cur_proc_state_by_prog (var_list, ps_map, ps_name) = (case (fmlookup ps_map ps_name) of Some (st) \<Rightarrow> st)"
+definition get_cur_proc_state_by_prog :: "program_state \<Rightarrow> process_state" where
+"get_cur_proc_state_by_prog ps = (case (fmlookup (fst (snd ps)) (snd (snd ps))) of Some (st) \<Rightarrow> st)"
 
 text "Getting process vars list in current process from program state"
 definition get_cur_proc_var_list :: "program_state \<Rightarrow>stacked_proc_var list" where 
@@ -45,14 +51,16 @@ definition get_cur_proc_var_list :: "program_state \<Rightarrow>stacked_proc_var
       proc_var_list)"
 
 text "Getting current program state from model state"
-fun get_cur_prog_state :: "model_state \<Rightarrow> program_state" where
-"get_cur_prog_state (ST global_var_decl_list (ps_map,p_name) function_block_decl_list function_decl_list) = 
-  (case (fmlookup ps_map p_name) of 
-    Some(p_state) \<Rightarrow> p_state)"
+definition get_cur_prog_state :: "model_state \<Rightarrow> program_state" where
+"get_cur_prog_state st = 
+  (case st of 
+    (ST global_var_decl_list (ps_map,p_name) function_block_decl_list function_decl_list) \<Rightarrow>
+      (case (fmlookup ps_map p_name) of 
+        Some(p_state) \<Rightarrow> p_state))"
 
 text "Getting program state by program name from model state"
-fun get_proc_state_by_prog :: "program_state \<Rightarrow> process_name \<Rightarrow> process_state" where
-"get_proc_state_by_prog (var_list, ps_map,ps_name) var_name = (case (fmlookup ps_map var_name) of Some (st) \<Rightarrow> st)"
+definition get_proc_state_by_prog :: "program_state \<Rightarrow> process_name \<Rightarrow> process_state" where
+"get_proc_state_by_prog ps var_name = (case (fmlookup (fst (snd ps)) var_name) of Some (st) \<Rightarrow> st)"
 
 text "Getting process state by process name from model state" 
 definition get_proc_state :: "model_state \<Rightarrow> process_name \<Rightarrow> process_state" where 
@@ -108,21 +116,28 @@ primrec set_symbvar_in_ps_in_var_list :: "(stacked_proc_var list) \<Rightarrow> 
 )) "
 
 text "Setting in process state new var init value by name"
-fun set_symbvar_in_ps :: "process_state \<Rightarrow> symbolic_var \<Rightarrow> stacked_var_init \<Rightarrow> process_state" where
-"set_symbvar_in_ps (proc_var_list, state_name, proc_stat, cur_time) var_name value = 
-  (set_symbvar_in_ps_in_var_list proc_var_list var_name value,state_name,proc_stat,cur_time)"
+definition set_symbvar_in_ps :: "process_state \<Rightarrow> symbolic_var \<Rightarrow> stacked_var_init \<Rightarrow> process_state" where
+"set_symbvar_in_ps ps var_name value = 
+  (set_symbvar_in_ps_in_var_list (fst ps) var_name value, (fst (snd ps)), (fst (snd (snd ps))), (snd (snd (snd ps))))"
 
 text "Setting in program state in current process new var value by name" 
-fun set_symbvar_in_ps_in_cur_proc :: "program_state \<Rightarrow> symbolic_var \<Rightarrow> stacked_var_init \<Rightarrow> program_state" where
-"set_symbvar_in_ps_in_cur_proc (var_list, proc_map, proc_name) var_name value = 
-  (case (fmlookup proc_map proc_name) of 
-    Some(proc_state) \<Rightarrow> (var_list,fmupd proc_name (set_symbvar_in_ps proc_state var_name value) proc_map,proc_name))"
+definition set_symbvar_in_ps_in_cur_proc :: "program_state \<Rightarrow> symbolic_var \<Rightarrow> stacked_var_init \<Rightarrow> program_state" where
+"set_symbvar_in_ps_in_cur_proc ps var_name value = 
+  (case (fmlookup (fst (snd ps)) (snd (snd ps))) of 
+    Some(proc_state) \<Rightarrow> ((fst ps), fmupd (snd (snd ps)) (set_symbvar_in_ps proc_state var_name value) (fst (snd ps)), (snd (snd ps))))"
 
 text "Setting in model state in current program new var init value by name"
-fun set_symbvar_in_ps_in_cur_prog :: "model_state \<Rightarrow> symbolic_var \<Rightarrow> stacked_var_init \<Rightarrow> model_state" where 
-"set_symbvar_in_ps_in_cur_prog (ST global_var_decl_list (ps_map,p_name) function_block_decl_list function_decl_list) var_name value = 
-  (case (fmlookup ps_map p_name) of
-    Some(p_state) \<Rightarrow> (ST global_var_decl_list ((fmupd p_name p_state ps_map), p_name) function_block_decl_list function_decl_list))"
+definition set_symbvar_in_ps_in_cur_prog :: "model_state \<Rightarrow> symbolic_var \<Rightarrow> stacked_var_init \<Rightarrow> model_state" where 
+"set_symbvar_in_ps_in_cur_prog st var_name value = 
+  (case st of 
+    (ST global_var_decl_list (ps_map,p_name) function_block_decl_list function_decl_list) \<Rightarrow>
+      (case (fmlookup ps_map p_name) of
+        Some(p_state) \<Rightarrow> 
+          (ST global_var_decl_list 
+            ((fmupd p_name (set_symbvar_in_ps_in_cur_proc p_state var_name value) ps_map), p_name) 
+            function_block_decl_list function_decl_list)))"
+
+print_theorems
 
 text "Setting in model state new symbolic var value by name"
 definition set_symbvar :: "model_state \<Rightarrow> symbolic_var \<Rightarrow> basic_post_type => model_state" where
@@ -157,12 +172,13 @@ definition check_proc_status :: "model_state \<Rightarrow> process_name \<Righta
     in (basic_post_type.Bool (proc_status_is cur_proc_stat proc_stat)))"
 
 text "Resetting timer in current process in model state"
-fun reset_timer :: "model_state \<Rightarrow> model_state" where
-"reset_timer (ST g_list (pr_map,pr_name) fb_list f_list) = 
-  (let (var_list, p_map,p_name) = (get_cur_prog_state (ST g_list (pr_map,pr_name) fb_list f_list));
-       (process_vars, current_state, start_state, process_status, t) = (get_cur_proc_state_by_prog (var_list,p_map,p_name))
-    in (ST 
-          g_list 
+definition reset_timer :: "model_state \<Rightarrow> model_state" where
+"reset_timer st = 
+  (case st of
+    (ST g_list (pr_map,pr_name) fb_list f_list) \<Rightarrow>
+      (let (var_list, p_map,p_name) = (get_cur_prog_state (ST g_list (pr_map,pr_name) fb_list f_list));
+           (process_vars, current_state, start_state, process_status, t) = (get_cur_proc_state_by_prog (var_list,p_map,p_name))
+        in (ST g_list 
           ((fmupd 
               pr_name 
               (var_list,(fmupd 
@@ -170,36 +186,37 @@ fun reset_timer :: "model_state \<Rightarrow> model_state" where
                  (process_vars, current_state, start_state, process_status, t)
                  p_map),p_name)
               pr_map),
-            pr_name) 
-          fb_list 
-          f_list))"
+            pr_name) fb_list f_list)))"
 
 text "Stopping process by name in model state"
-fun stop_process :: "model_state \<Rightarrow> process_name \<Rightarrow> model_state" where
-"stop_process (ST global_var_decl_list (ps_map,p_name) function_block_decl_list function_decl_list) target_proc_name =
-   (let (var_list,proc_map, proc_name) = (case (fmlookup ps_map p_name) of 
-                              Some(p_state) \<Rightarrow> p_state);
-        ((proc_var_list), st_name,start_st_name, proc_stat, cur_time) = (case (fmlookup proc_map target_proc_name) of 
-                                    Some(proc_state) \<Rightarrow> proc_state)
-    in (ST 
-        global_var_decl_list 
+definition stop_process :: "model_state \<Rightarrow> process_name \<Rightarrow> model_state" where
+"stop_process st target_proc_name =
+   (case st of 
+    (ST global_var_decl_list (ps_map,p_name) function_block_decl_list function_decl_list) \<Rightarrow>
+      (let (var_list,proc_map, proc_name) = 
+        (case (fmlookup ps_map p_name) of
+          Some(p_state) \<Rightarrow> p_state);
+        ((proc_var_list), st_name,start_st_name, proc_stat, cur_time) = 
+          (case (fmlookup proc_map target_proc_name) of 
+            Some(proc_state) \<Rightarrow> proc_state)
+        in (ST global_var_decl_list 
         ((fmupd 
             p_name
             (var_list,
-(fmupd 
-                 target_proc_name
-                 ((proc_var_list), st_name,start_st_name, proc_status.Stop, cur_time)
-                 proc_map), 
+              (fmupd 
+                target_proc_name
+                ((proc_var_list), st_name,start_st_name, proc_status.Stop, cur_time)
+                proc_map), 
               proc_name) 
             ps_map),
-          p_name) 
-        function_block_decl_list 
-        function_decl_list))"
+          p_name) function_block_decl_list function_decl_list)))"
 
 text "Stopping current process in model state"
-fun stop_same_process :: "model_state  \<Rightarrow> model_state" where
-"stop_same_process (ST global_var_decl_list (ps_map,p_name) function_block_decl_list function_decl_list) =
-   (let (var_list,proc_map, proc_name) = (case (fmlookup ps_map p_name) of 
+definition stop_same_process :: "model_state  \<Rightarrow> model_state" where
+"stop_same_process st =
+  (case st of
+    (ST global_var_decl_list (ps_map,p_name) function_block_decl_list function_decl_list) \<Rightarrow>
+(let (var_list,proc_map, proc_name) = (case (fmlookup ps_map p_name) of
                               Some(p_state) \<Rightarrow> p_state);
         ((proc_var_list), st_name,start_st_name, proc_stat, cur_time) = (case (fmlookup proc_map proc_name) of 
                                     Some(proc_state) \<Rightarrow> proc_state)
@@ -215,12 +232,14 @@ fun stop_same_process :: "model_state  \<Rightarrow> model_state" where
             ps_map),
           p_name) 
         function_block_decl_list 
-        function_decl_list)) "
+        function_decl_list)))"
 
 text "Erroring process by name in model state"
-fun error_process :: "model_state \<Rightarrow> process_name \<Rightarrow> model_state" where
-"error_process (ST global_var_decl_list (ps_map,p_name) function_block_decl_list function_decl_list) target_proc_name =
-   (let (var_list,proc_map, proc_name) = (case (fmlookup ps_map p_name) of 
+definition error_process :: "model_state \<Rightarrow> process_name \<Rightarrow> model_state" where
+"error_process st target_proc_name =
+   (case st of 
+      (ST global_var_decl_list (ps_map,p_name) function_block_decl_list function_decl_list) \<Rightarrow>
+(let (var_list,proc_map, proc_name) = (case (fmlookup ps_map p_name) of
                               Some(p_state) \<Rightarrow> p_state);
         ((proc_var_list), st_name,start_st_name, proc_stat, cur_time) = (case (fmlookup proc_map target_proc_name) of 
                                     Some(proc_state) \<Rightarrow> proc_state)
@@ -236,12 +255,14 @@ fun error_process :: "model_state \<Rightarrow> process_name \<Rightarrow> model
             ps_map),
           p_name) 
         function_block_decl_list 
-        function_decl_list))"
+        function_decl_list)))"
 
 text "Erroring current process in model state"
-fun error_same_process :: "model_state \<Rightarrow> model_state" where
-"error_same_process (ST global_var_decl_list (ps_map,p_name) function_block_decl_list function_decl_list) =
-   (let (var_list,proc_map, proc_name) = (case (fmlookup ps_map p_name) of 
+definition error_same_process :: "model_state \<Rightarrow> model_state" where
+"error_same_process st =
+   (case st of 
+(ST global_var_decl_list (ps_map,p_name) function_block_decl_list function_decl_list) \<Rightarrow>
+(let (var_list,proc_map, proc_name) = (case (fmlookup ps_map p_name) of
                               Some(p_state) \<Rightarrow> p_state);
         ((proc_var_list), st_name,start_st_name, proc_stat, cur_time) = (case (fmlookup proc_map proc_name) of 
                                     Some(proc_state) \<Rightarrow> proc_state)
@@ -257,12 +278,14 @@ fun error_same_process :: "model_state \<Rightarrow> model_state" where
             ps_map),
           p_name) 
         function_block_decl_list 
-        function_decl_list))"
+        function_decl_list)))"
 
 text "Resetting process by name in model state"
-fun reset_process :: "model_state \<Rightarrow> process_name \<Rightarrow> model_state" where
-"reset_process (ST global_var_decl_list (ps_map,p_name) function_block_decl_list function_decl_list) target_proc_name =
-  (let (var_list,proc_map, proc_name) = (case (fmlookup ps_map p_name) of 
+definition reset_process :: "model_state \<Rightarrow> process_name \<Rightarrow> model_state" where
+"reset_process st target_proc_name =
+  (case st of
+(ST global_var_decl_list (ps_map,p_name) function_block_decl_list function_decl_list) \<Rightarrow>
+(let (var_list,proc_map, proc_name) = (case (fmlookup ps_map p_name) of
                               Some(p_state) \<Rightarrow> p_state);
         ((proc_var_list), _ ,start_st_name, proc_stat, cur_time) = (case (fmlookup proc_map target_proc_name) of 
                                     Some(proc_state) \<Rightarrow> proc_state)
@@ -278,12 +301,14 @@ fun reset_process :: "model_state \<Rightarrow> process_name \<Rightarrow> model
             ps_map),
           p_name) 
         function_block_decl_list 
-        function_decl_list))"
+        function_decl_list)))"
 
 text "Resetting current process in model state"
-fun reset_same_process :: "model_state \<Rightarrow> model_state" where
-"reset_same_process (ST global_var_decl_list (ps_map,p_name) function_block_decl_list function_decl_list)  =
-  (let (var_list,proc_map, proc_name) = (case (fmlookup ps_map p_name) of 
+definition reset_same_process :: "model_state \<Rightarrow> model_state" where
+"reset_same_process st  =
+  (case st of 
+(ST global_var_decl_list (ps_map,p_name) function_block_decl_list function_decl_list) \<Rightarrow>
+(let (var_list,proc_map, proc_name) = (case (fmlookup ps_map p_name) of
                               Some(p_state) \<Rightarrow> p_state);
         ((proc_var_list), _,start_st_name, proc_stat, cur_time) = (case (fmlookup proc_map proc_name) of 
                                     Some(proc_state) \<Rightarrow> proc_state)
@@ -299,12 +324,14 @@ fun reset_same_process :: "model_state \<Rightarrow> model_state" where
             ps_map),
           p_name) 
         function_block_decl_list 
-        function_decl_list))"
+        function_decl_list)))"
 
 text "Setting new state by name in current process in model state"
-fun set_state :: "model_state \<Rightarrow> state_name \<Rightarrow> model_state" where
-"set_state (ST global_var_decl_list (ps_map,p_name) function_block_decl_list function_decl_list) st_name = 
-  (let (var_list,proc_map, proc_name) = (case (fmlookup ps_map p_name) of 
+definition set_state :: "model_state \<Rightarrow> state_name \<Rightarrow> model_state" where
+"set_state st st_name = 
+  (case st of
+(ST global_var_decl_list (ps_map,p_name) function_block_decl_list function_decl_list) \<Rightarrow>
+(let (var_list,proc_map, proc_name) = (case (fmlookup ps_map p_name) of
                               Some(p_state) \<Rightarrow> p_state);
         ((proc_var_list), _ ,start_st_name, proc_stat, cur_time) = (case (fmlookup proc_map proc_name) of 
                                     Some(proc_state) \<Rightarrow> proc_state)
@@ -320,34 +347,40 @@ fun set_state :: "model_state \<Rightarrow> state_name \<Rightarrow> model_state
             ps_map),
           p_name) 
         function_block_decl_list 
-        function_decl_list))"
+        function_decl_list)))"
 
 text "Extracting new process state from stacked process"
-fun extract_process_state :: "stacked_process \<Rightarrow> process_state" where
-"extract_process_state (proc_name, var_list,((name, _, _, _)#other)) = 
-  (var_list, name, name, proc_status.Inactive, (time.Time 0 0 0 0 0))"
+definition extract_process_state :: "stacked_process \<Rightarrow> process_state" where
+"extract_process_state sp  = 
+  (case sp of 
+    (proc_name, var_list,((name, _, _, _)#other)) \<Rightarrow> 
+    (var_list, name, name, proc_status.Inactive, (time.Time 0 0 0 0 0)))"
 
 
 text "Extracting new program state from stacked program"
-fun extract_program_state :: "stacked_program \<Rightarrow> program_state" where 
-"extract_program_state (prog_name, var_list, st_proc_list) =
-  (let (name,_,_) = (nth st_proc_list 0);
+definition extract_program_state :: "stacked_program \<Rightarrow> program_state" where 
+"extract_program_state sp =
+  (case sp of
+    (prog_name, var_list, st_proc_list) \<Rightarrow>
+      (let (name,_,_) = (nth st_proc_list 0);
        proc_states = (fmap_of_list 
                         (map 
                           (\<lambda>(proc_name,var_list,state_list). 
                             (proc_name,(extract_process_state (proc_name,var_list,state_list)))) 
                           st_proc_list))
-    in (var_list,proc_states,name))"
+    in (var_list,proc_states,name)))"
 
 text "Extracting new model state from stacked model"
-fun extract_model_state :: "stacked_model \<Rightarrow> model_state" where
-"extract_model_state (conf, global, prog_list, fb_list, f_list) =
-  (let (name, _, _) = (nth prog_list 0); 
+definition extract_model_state :: "stacked_model \<Rightarrow> model_state" where
+"extract_model_state sm =
+  (case sm of 
+    (conf, global, prog_list, fb_list, f_list) \<Rightarrow>
+(let (name, _, _) = (nth prog_list 0);
         prog_map = (fmap_of_list
     (map
       (\<lambda>(name, var_list, proc_list). (name, (extract_program_state (name, var_list, proc_list))))
       prog_list))
-  in (model_state.ST global (prog_map,name) fb_list f_list))"
+  in (model_state.ST global (prog_map,name) fb_list f_list)))"
 
 
 end
